Source/IntegrationTests/TestFiles/LitTests/LitTest/comp/placeholders/complex/user.dfy
@@ -2,11 +2,14 @@
 // RUN: %baredafny run %args %s --build=%S/Build/build --input %S/Inputs/wrappers.dfy --input %S/Inputs/random.dfy --input %S/Inputs/randomCSharp.dfy --input %S/Inputs/Interop.cs >> "%t"
 // RUN: %diff "%s.expect" "%t"
 
+// Test can fail non-deterministically by design, but the chance is ~10^-30
 method Main() {
   var x := DfyRandom.GetRandomNat(1000000);
   var y := 0;
   var i := 5;
-  while(x != y && i != 0) {
+  while(x != y && i != 0)
+    decreases i
+  {
     y := DfyRandom.GetRandomNat(1000000);
     i := i - 1;
   }
